BlockCoordinationSystemRefinement RefinementInit

Splinter/BlockLayer/BlockCoordinationSystem.i.dfy
@@ -65,6 +65,11 @@ module BlockCoordinationSystem
     }
   }
 
+  function MkfsDiskImage() : DiskImage
+  {
+    DiskImage(StampedMapMod.Empty(), MarshalledJournal.Mkfs())
+  }
+
   datatype Variables = Variables(
     persistentImage: DiskImage,
     ephemeral: Ephemeral,
@@ -75,6 +80,13 @@ module BlockCoordinationSystem
       && persistentImage.WF()
       && (ephemeral.Known? ==> ephemeral.WF())
       && (inFlightImage.Some? ==> inFlightImage.value.WF())
+    }
+
+    predicate Init()
+    {
+      && persistentImage == MkfsDiskImage()
+      && ephemeral.Unknown?
+      && inFlightImage.None?
     }
   }
 
