Splinter/BlockLayer/BlockCoordinationSystemRefinement.i.dfy
@@ -1,0 +1,106 @@
+// Copyright 2018-2021 VMware, Inc., Microsoft Inc., Carnegie Mellon University, ETH Zurich, and University of Washington
+// SPDX-License-Identifier: BSD-2-Clause
+
+include "BlockCoordinationSystem.i.dfy"
+include "../CoordinationLayer/CoordinationSystem.i.dfy"
+
+module BlockCoordinationSystemRefinement
+{
+  import opened Options
+  import opened BlockCoordinationSystem
+  import MarshalledJournal
+  import CoordinationSystem
+  import AbstractJournal
+  import opened MsgHistoryMod
+  import LinkedJournal
+
+  predicate JournalImageInv(journalImage: MarshalledJournal.JournalImage)
+  {
+    && journalImage.WF()
+    && journalImage.I().diskView.Acyclic()
+    && journalImage.I().I().WF()
+  }
+
+  predicate DiskImageInv(diskImage: DiskImage)
+  {
+    && JournalImageInv(diskImage.journal)
+  }
+
+  predicate MarshalledJournalInv(v: MarshalledJournal.Variables)
+  {
+    && JournalImageInv(v.journalImage)
+    && v.unmarshalledTail.WF()
+    && JournalImageI(v.journalImage).CanConcat(v.unmarshalledTail)
+  }
+
+  predicate EphemeralInv(ephemeral: Ephemeral)
+  {
+    && (ephemeral.Known? ==> MarshalledJournalInv(ephemeral.journal))
+  }
+
+  predicate Inv(v: Variables)
+  {
+    && DiskImageInv(v.persistentImage)
+    && EphemeralInv(v.ephemeral)
+    && (v.inFlightImage.Some? ==> DiskImageInv(v.inFlightImage.value))
+  }
+
+  function JournalImageI(journalImage: MarshalledJournal.JournalImage) : MsgHistory
+    requires JournalImageInv(journalImage)
+  {
+    journalImage.I().I().I()
+  }
+
+  function DiskImageI(diskImage: DiskImage) : CoordinationSystem.DiskImage
+    requires DiskImageInv(diskImage)
+  {
+    CoordinationSystem.DiskImage(diskImage.mapadt, JournalImageI(diskImage.journal))
+  }
+
+  function MarshalledJournalI(v: MarshalledJournal.Variables) : AbstractJournal.Variables
+    requires MarshalledJournalInv(v)
+  {
+    AbstractJournal.Variables(JournalImageI(v.journalImage).Concat(v.unmarshalledTail))
+  }
+
+  function EphemeralI(ephemeral: Ephemeral) : CoordinationSystem.Ephemeral
+    requires EphemeralInv(ephemeral)
+  {
+    if ephemeral.Unknown? then
+      CoordinationSystem.Unknown
+    else
+      CoordinationSystem.Known(
+      ephemeral.progress,
+      ephemeral.syncReqs,
+      ephemeral.mapadt,
+      ephemeral.mapLsn,
+      MarshalledJournalI(ephemeral.journal),
+      ephemeral.frozenMap
+      )
+  }
+
+  function I(v: Variables) : CoordinationSystem.Variables
+    requires Inv(v)
+  {
+    CoordinationSystem.Variables(
+      DiskImageI(v.persistentImage),
+      EphemeralI(v.ephemeral),
+      if v.inFlightImage.Some? then Some(DiskImageI(v.inFlightImage.value)) else None
+      )
+  }
+
+  lemma RefinementInit(v: Variables)
+    requires v.Init()
+    ensures Inv(v)
+    ensures I(v).Init()
+  {
+    assert v.persistentImage.journal.TypeProvidesModel(LinkedJournal.Mkfs());
+    assert v.persistentImage.journal.I().diskView.PointersRespectRank(map[]);
+  }
+
+  lemma RefinementNext(v: Variables, v': Variables, uiop: UIOp)
+    requires Inv(v)
+    requires Next(v, v', uiop)
+    ensures Inv(v')
+    ensures CoordinationSystem.Next(I(v), I(v'), uiop)
+}
